\begin{circuitikz}
	\draw (0, 0) node[gyrator] (G) {};
	\draw (G.base) node{$G_D$};
  	\draw ($(G.A1) - (1, 0)$) node[left] {$U_\alpha$} to[short,o-,i=$i_1$] (G.A1);
  	\draw (G.A2) to[short,-o] ($(G.A2) - (1, 0)$) node[left] {$U_\beta$};
  	\draw ($(G.B1) + (1, 0)$) node[right] {$U_\gamma$} to[short,o-,i=$i_2$] (G.B1);
  	\draw (G.B2) to[short,-o] ($(G.B2) + (1, 0)$) node[right] {$U_\delta$};
  	\draw ($(G.A2) - (1, 0)$) to[open,v^=$u_1$] ($(G.A1) - (1, 0)$);
  	\draw ($(G.B2) + (1, 0)$) to[open,v=$u_2$] ($(G.B1) + (1, 0)$);
\end{circuitikz}